thy/OpenFlow/OpenFlowMatches.thy
@@ -106,7 +106,7 @@ definition "simple_packet_unext p =
 p_sport = p_sport p, p_dport = p_dport p, p_tcp_flags = p_tcp_flags p, p_tag_ctstate = p_tag_ctstate p\<rparr>"
 
 
-fun match_no_prereq :: "of_match_field \<Rightarrow> simple_packet_ext \<Rightarrow> bool" where
+fun match_no_prereq :: "of_match_field \<Rightarrow> 'a simple_packet_ext_scheme \<Rightarrow> bool" where
 "match_no_prereq (IngressPort i) p = (p_iiface p = i)" |
 "match_no_prereq (EtherDst i) p = (p_l2src p = i)" |
 "match_no_prereq (EtherSrc i) p = (p_l2dst p = i)" |
@@ -119,14 +119,14 @@ fun match_no_prereq :: "of_match_field \<Rightarrow> simple_packet_ext \<Rightar
 "match_no_prereq (L4Src i m) p = (p_sport p && m = i)" |
 "match_no_prereq (L4Dst i m) p = (p_dport p && m = i)"
 
-definition match_prereq :: "of_match_field \<Rightarrow> of_match_field set \<Rightarrow> simple_packet_ext \<Rightarrow> bool option" where
+definition match_prereq :: "of_match_field \<Rightarrow> of_match_field set \<Rightarrow> 'a simple_packet_ext_scheme \<Rightarrow> bool option" where
 "match_prereq i s p = (if prerequisites i s then Some (match_no_prereq i p) else None)"
 
 definition "set_seq s \<equiv> if (\<forall>x \<in> s. x \<noteq> None) then Some (the ` s) else None"
 definition "all_true s \<equiv> \<forall>x \<in> s. x"
 term map_option
-definition OF_match_fields :: "of_match_field set \<Rightarrow> simple_packet_ext \<Rightarrow> bool option" where "OF_match_fields m p = map_option all_true (set_seq ((\<lambda>f. match_prereq f m p) ` m))"
-definition OF_match_fields_unsafe :: "of_match_field set \<Rightarrow> simple_packet_ext \<Rightarrow> bool" where "OF_match_fields_unsafe m p = (\<forall>f \<in> m. match_no_prereq f p)"
+definition OF_match_fields :: "of_match_field set \<Rightarrow> 'a simple_packet_ext_scheme \<Rightarrow> bool option" where "OF_match_fields m p = map_option all_true (set_seq ((\<lambda>f. match_prereq f m p) ` m))"
+definition OF_match_fields_unsafe :: "of_match_field set \<Rightarrow> 'a simple_packet_ext_scheme \<Rightarrow> bool" where "OF_match_fields_unsafe m p = (\<forall>f \<in> m. match_no_prereq f p)"
 
 definition "all_prerequisites m \<equiv> \<forall>f \<in> m. prerequisites f m"
 
