thy/Routing/LinuxRouter.thy
@@ -34,13 +34,13 @@ term simple_fw
 definition simple_linux_router :: "routing_rule list \<Rightarrow> simple_rule list \<Rightarrow> (32 word \<Rightarrow> 48 word option) \<Rightarrow> interface list \<Rightarrow> simple_packet_ext \<Rightarrow> simple_packet_ext option" where
 "simple_linux_router rt fw mlf ifl p \<equiv> do {
 	_ \<leftarrow> iface_packet_check ifl p;
-	let rd = routing_table_semantics rt (p_dst p);
-	let p = p_oiface_update (const (output_iface rd)) p;
-	let fd = simple_fw fw p;
+	let rd (* routing decision *) = routing_table_semantics rt (p_dst p);
+	let p = p\<lparr>p_oiface := output_iface rd\<rparr>;
+	let fd (* firewall decision *) = simple_fw fw p;
+	_ \<leftarrow> (case fd of Decision FinalAllow \<Rightarrow> Some () | Decision FinalDeny \<Rightarrow> None);
 	let nh = fromMaybe (p_dst p) (next_hop rd);
 	ma \<leftarrow> mlf nh;
-	_ \<leftarrow> (case fd of Decision FinalAllow \<Rightarrow> Some () | Decision FinalDeny \<Rightarrow> None);
-	Some (p_l2dst_update (const ma) p)
+	Some (p\<lparr>p_l2dst := ma\<rparr>)
 }"
 (* Can I find something that looks a bit more semantic. Maybe the option monad can reduce a bit of the foo? *)
 (* TODO: What happens in linux, if I send a packet to an interface with the mac of another interface? Hopefully, that is going to be dropped? *) 
@@ -57,7 +57,7 @@ text{* Transformed linux router: does not do layer 2 modifications and throws aw
 definition simple_linux_router_nomac :: "routing_rule list \<Rightarrow> simple_rule list \<Rightarrow> 'a simple_packet_scheme \<Rightarrow> 'a simple_packet_scheme option" where
 "simple_linux_router_nomac rt fw p \<equiv> do {
 	let rd = routing_table_semantics rt (p_dst p);
-	_ \<leftarrow> (if output_iface rd = p_oiface p then None else Some ());
+	_ \<leftarrow> (if output_iface rd = p_iiface p then None else Some ());
 	let p = p_oiface_update (const (output_iface rd)) p;
 	let fd = simple_fw fw p;
 	_ \<leftarrow> (case fd of Decision FinalAllow \<Rightarrow> Some () | Decision FinalDeny \<Rightarrow> None);
@@ -76,7 +76,7 @@ by(simp add: Let_def split: option.splits state.splits final_decision.splits Opt
 
 lemma rtr_nomac_e2:
 	assumes "simple_linux_router rt fw mlf ifl pi = Some po"
-	assumes "p_oiface pi \<noteq> p_oiface po"
+	assumes "p_iiface pi \<noteq> p_iiface po"
 	shows "\<exists>po'. simple_linux_router_nomac rt fw pi = Some po'"
 using assms
 unfolding simple_linux_router_nomac_def simple_linux_router_def
@@ -92,8 +92,8 @@ unfolding simple_linux_router_nomac_def simple_linux_router_def
 by(clarsimp simp add: Let_def const_def split: option.splits state.splits final_decision.splits Option.bind_splits if_splits)
 
 lemma rtr_nomac_eq:
-	assumes "iface_packet_check ifl pi = None \<longleftrightarrow> output_iface (routing_table_semantics rt (p_dst pi)) = p_oiface pi"
-	assumes "mlf (fromMaybe (p_dst pi) (next_hop (routing_table_semantics rt (p_dst pi)))) = Some i2"
+	assumes "iface_packet_check ifl pi = None \<longleftrightarrow> output_iface (routing_table_semantics rt (p_dst pi)) = p_iiface pi"
+	assumes "mlf (fromMaybe (p_dst pi) (next_hop (routing_table_semantics rt (p_dst pi)))) \<noteq> None"
 	shows "\<exists>x. map_option (p_l2dst_update x) (simple_linux_router_nomac rt fw pi) = simple_linux_router rt fw mlf ifl pi"
 proof(cases "simple_linux_router_nomac rt fw pi"; cases "simple_linux_router rt fw mlf ifl pi")
 	case goal4
@@ -102,7 +102,7 @@ proof(cases "simple_linux_router_nomac rt fw pi"; cases "simple_linux_router rt 
 next
 	case (goal2 a)
 	from goal2(2) have "iface_packet_check ifl pi \<noteq> None" by(simp add: simple_linux_router_def Let_def const_def split: option.splits state.splits final_decision.splits Option.bind_splits if_splits) 
-	hence "p_oiface pi \<noteq> p_oiface a" using assms(1) goal2(2) by(clarsimp simp add: simple_linux_router_def Let_def const_def split: option.splits state.splits final_decision.splits Option.bind_splits if_splits)
+	hence "p_iiface pi \<noteq> p_iiface a" using assms(1) goal2(2) sorry by(clarsimp simp add: simple_linux_router_def Let_def const_def split: option.splits state.splits final_decision.splits Option.bind_splits if_splits)
 	note rtr_nomac_e2[OF goal2(2) this]
 	with goal2(1) have False by simp
 	thus ?case ..
@@ -121,8 +121,8 @@ qed simp
 
 lemma rtr_nomac_eq_halfinv:
 	assumes fw_ac_all: "fw = [SimpleRule simple_match_any Accept]"
-	assumes a1: "\<exists>x. map_option (p_l2dst_update x) (simple_linux_router_nomac rt fw pi) = simple_linux_router rt fw mlf ifl pi"
-	assumes a2: "mlf (fromMaybe (p_dst pi) (next_hop (routing_table_semantics rt (p_dst pi)))) = Some i2"
+	assumes a1: "\<exists>dst_mac_f. map_option (p_l2dst_update dst_mac_f) (simple_linux_router_nomac rt fw pi) = simple_linux_router rt fw mlf ifl pi"
+	assumes a2: "mlf (fromMaybe (p_dst pi) (next_hop (routing_table_semantics rt (p_dst pi)))) \<noteq> None"
 	shows "iface_packet_check ifl pi = None \<longleftrightarrow> output_iface (routing_table_semantics rt (p_dst pi)) = p_oiface pi"
 using a1 a2
 	apply(clarify)
@@ -130,5 +130,17 @@ using a1 a2
 	apply(unfold fw_ac_all)
 	apply(simp_all add: simple_linux_router_nomac_def simple_linux_router_def Let_def simple_match_any split: Option.bind_splits if_splits)
 done
+
+lemma rtr_nomac_eq_halfinv_noexquant:
+	assumes fw_ac_all: "fw = [SimpleRule simple_match_any Accept]"
+	assumes a1: "map_option (p_l2dst_update (const dst_mac)) (simple_linux_router_nomac rt fw pi) = simple_linux_router rt fw mlf ifl pi"
+	assumes a2: "mlf (fromMaybe (p_dst pi) (next_hop (routing_table_semantics rt (p_dst pi)))) = Some dst_mac"
+	shows "iface_packet_check ifl pi = None \<longleftrightarrow> output_iface (routing_table_semantics rt (p_dst pi)) = p_oiface pi"
+using a1 a2 unfolding const_def
+	apply(cases "simple_linux_router rt fw mlf ifl pi")
+	apply(unfold fw_ac_all)
+	apply(simp_all add: simple_linux_router_nomac_def simple_linux_router_def Let_def simple_match_any split: Option.bind_splits if_splits)
+done
+sorry
 
 end
